Move erasure wcbv eval into Type

erasure/theories/EWcbvEval.v
@@ -80,7 +80,7 @@ Section Wcbv.
   Context (Σ : global_declarations).
   (* The local context is fixed: we are only doing weak reductions *)
 
-  Inductive eval : term -> term -> Prop :=
+  Inductive eval : term -> term -> Type :=
   (** Reductions *)
   | eval_box a t t' :
       eval a tBox ->
@@ -193,36 +193,47 @@ Section Wcbv.
   Definition value_head x :=
     isConstruct x || isCoFix x.
 
-  Inductive value : term -> Prop :=
+  Inductive value : term -> Type :=
   | value_atom t : atom t -> value t
   (* | value_evar n l l' : Forall value l -> Forall value l' -> value (mkApps (tEvar n l) l') *)
-  | value_app t l : value_head t -> Forall value l -> value (mkApps t l)
+  | value_app t l : value_head t -> All value l -> value (mkApps t l)
   | value_stuck_fix f args :
-      Forall value args ->
+      All value args ->
       isStuckFix f args ->
-      value (mkApps f args)
-  .
+      value (mkApps f args).
+  
 
-  Lemma value_values_ind : forall P : term -> Prop,
+  Lemma value_values_rect : forall P : term -> Type,
       (forall t, atom t -> P t) ->
-      (forall t l, value_head t -> Forall value l -> Forall P l -> P (mkApps t l)) ->
+      (forall t l, value_head t -> All value l -> All P l -> P (mkApps t l)) ->
       (forall f args,
-          Forall value args ->
-          Forall P args ->
+          All value args ->
+          All P args ->
           isStuckFix f args ->
           P (mkApps f args)) ->
       forall t : term, value t -> P t.
   Proof.
     intros P ? ? ?.
     fix value_values_ind 2. destruct 1.
-    - apply H; auto.
-    - eapply H0; auto.
-      revert l H3. fix aux 2. destruct 1. constructor; auto.
+    - apply X; auto.
+    - eapply X0; auto.
+      revert l a. fix aux 2. destruct 1. constructor; auto.
       constructor. eauto. eauto.
-    - eapply H1; eauto.
-      clear H3. revert args H2. fix aux 2. destruct 1. constructor; auto.
+    - eapply X1; eauto.
+      clear i. revert args a. fix aux 2. destruct 1. constructor; auto.
       constructor. now eapply value_values_ind. now apply aux.
   Defined.
+
+  Lemma value_values_ind : forall P : term -> Prop,
+      (forall t, atom t -> P t) ->
+      (forall t l, value_head t -> All value l -> Forall P l -> P (mkApps t l)) ->
+      (forall f args,
+          All value args ->
+          Forall P args ->
+          isStuckFix f args ->
+          P (mkApps f args)) ->
+      forall t : term, value t -> P t.
+  Proof. intros; apply value_values_rect; eauto using All_Forall. Defined.
 
   Lemma value_head_nApp {t} : value_head t -> ~~ isApp t.
   Proof. destruct t; auto. Qed.
@@ -239,9 +250,9 @@ Section Wcbv.
   Lemma value_mkApps_inv t l :
     ~~ isApp t ->
     value (mkApps t l) ->
-    ((l = []) /\ atom t) \/ (value_head t /\ Forall value l) \/ (isStuckFix t l /\ Forall value l).
+    ((l = []) * atom t) + (value_head t * All value l) + (isStuckFix t l * All value l).
   Proof.
-    intros H H'. generalize_eqs H'. revert t H. induction H' using value_values_ind.
+    intros H H'. generalize_eqs H'. revert t H. induction H' using value_values_rect.
     intros.
     subst.
     - now eapply atom_mkApps in H.
@@ -280,44 +291,43 @@ Section Wcbv.
     - change (tApp ?h ?a) with (mkApps h [a]).
       rewrite mkApps_nested.
       apply value_mkApps_inv in IHeval1; [|easy].
-      destruct IHeval1 as [(-> & _)|[|(stuck & vals)]].
+      destruct IHeval1 as [[(-> & _)|]|(stuck & vals)].
       + cbn in *.
         apply (value_stuck_fix _ [av]); [easy|].
         cbn.
         destruct (cunfold_fix mfix idx) as [(? & ?)|]; [|easy].
-        noconf H1.
-        destruct H2 as [|(<- & ?)]; [|easy].
+        noconf e.
+        destruct o as [|(<- & ?)]; [|easy].
         unfold is_nth_constructor_app_or_box.
         now rewrite (proj2 (nth_error_None _ _));
           cbn in *.
       + easy.
-      + eapply value_stuck_fix; [now apply Forall_app_inv|].
+      + eapply value_stuck_fix; [now apply All_app_inv|].
         unfold isStuckFix in *.
         destruct (cunfold_fix mfix idx) as [(? & ?)|]; [|easy].
-        noconf H1.
+        noconf e.
         unfold is_nth_constructor_app_or_box in *.
-        destruct H2 as [|(<- & ?)]; [|now rewrite nth_error_snoc].
+        destruct o as [|(<- & ?)]; [|now rewrite nth_error_snoc].
         destruct (Nat.ltb_spec #|argsv| narg).
         * rewrite (proj2 (nth_error_None _ _)); [|easy].
           rewrite app_length.
           cbn.
           easy.
         * now rewrite nth_error_app1.
-
     - destruct (mkApps_elim f' [a']).
       eapply value_mkApps_inv in IHeval1 => //.
       destruct IHeval1; intuition subst.
-      * rewrite H3.
-        simpl. rewrite H3 in H. simpl in *.
-        apply (value_app f0 [a']). rewrite H3 in H0. destruct f0; simpl in * |- *; try congruence.
+      * rewrite a1.
+        simpl. rewrite a1 in H. simpl in *.
+        apply (value_app f0 [a']). rewrite a1 in i. destruct f0; simpl in * |- *; try congruence.
         constructor; auto. constructor. constructor; auto.
       * rewrite [tApp _ _](mkApps_nested _ (firstn n l) [a']).
-        constructor 2; auto. eapply Forall_app_inv; auto.
+        constructor 2; auto. eapply All_app_inv; auto.
       * rewrite [tApp _ _](mkApps_nested _ (firstn n l) [a']).
-        erewrite isFixApp_mkApps in H0 => //.
+        erewrite isFixApp_mkApps in i => //.
         destruct f0; simpl in *; try congruence.
         rewrite /isFixApp in H0. simpl in H0.
-        rewrite orb_true_r orb_true_l in H0. easy.
+        rewrite orb_true_r orb_true_l in i. easy.
   Qed.
 
   Lemma closed_unfold_fix_cunfold_eq mfix idx : 
@@ -430,7 +440,7 @@ Proof.
   - depelim ev'.
     + apply IHev1 in ev'1; solve_discr.
     + subst.
-      noconf H0.
+      noconf e0.
       now apply IHev2 in ev'2.
     + apply eval_mkApps_tCoFix in ev1 as (? & ?); solve_discr.
     + easy.
@@ -440,27 +450,26 @@ Proof.
     + apply IHev1 in ev'1.
       apply mkApps_eq_inj in ev'1; try easy.
       depelim ev'1.
-      noconf H2.
+      noconf H.
       subst.
       apply IHev2 in ev'2; subst.
-      rewrite H4 in H.
-      now noconf H.
+      rewrite e1 in e.
+      now noconf e.
     + apply IHev1 in ev'1.
       apply mkApps_eq_inj in ev'1; try easy.
       depelim ev'1.
-      noconf H2.
-      noconf H3.
+      noconf H.
       apply IHev2 in ev'2.
       subst.
-      rewrite H4 in H.
-      noconf H.
-      destruct H5 as [|(_ & ?)]; [easy|].
+      rewrite e1 in e.
+      noconf e.
+      destruct o as [|(_ & ?)]; [easy|].
       now apply negb_true_iff in H.
     + apply IHev1 in ev'1.
       subst.
-      rewrite isFixApp_mkApps in H2 by easy.
+      rewrite isFixApp_mkApps in i0 by easy.
       cbn in *.
-      now rewrite orb_true_r in H2.
+      now rewrite orb_true_r in i0.
     + easy.
   - depelim ev'.
     + apply IHev1 in ev'1; solve_discr.
@@ -470,33 +479,33 @@ Proof.
       apply mkApps_eq_inj in ev'1 as (ev'1 & <-); try easy.
       noconf ev'1.
       subst.
-      rewrite H1 in H.
-      noconf H.
-      destruct H0 as [|(? & ?)]; [easy|].
+      rewrite e0 in e.
+      noconf e.
+      destruct o as [|(? & ?)]; [easy|].
       now apply negb_true_iff in H0.
     + apply IHev1 in ev'1.
       apply IHev2 in ev'2.
       now apply mkApps_eq_inj in ev'1 as (ev'1 & <-).
     + apply IHev1 in ev'1.
       subst.
-      rewrite isFixApp_mkApps in H1 by easy.
-      cbn in H1.
-      now rewrite orb_true_r in H1.
+      rewrite isFixApp_mkApps in i by easy.
+      cbn in i.
+      now rewrite orb_true_r in i.
     + easy.
   - depelim ev'.
     + apply eval_mkApps_tCoFix in ev'1 as (? & ?); solve_discr.
     + apply eval_mkApps_tCoFix in ev'1 as (? & ?); solve_discr.
-    + apply mkApps_eq_inj in H1 as (H1 & <-); try easy.
+    + apply mkApps_eq_inj in H as (H1 & <-); try easy.
       noconf H1.
-      rewrite H0 in H.
-      noconf H.
+      rewrite e0 in e.
+      noconf e.
       now apply IHev in ev'.
     + easy.
   - depelim ev'.
-    + apply mkApps_eq_inj in H1 as (H1 & <-); try easy.
+    + apply mkApps_eq_inj in H as (H1 & <-); try easy.
       noconf H1.
-      rewrite H0 in H.
-      noconf H.
+      rewrite e0 in e.
+      noconf e.
       now apply IHev in ev'.
     + apply eval_mkApps_tCoFix in ev'1 as (? & ?); solve_discr.
     + apply eval_mkApps_tCoFix in ev' as (? & ?); solve_discr.
@@ -505,8 +514,8 @@ Proof.
     + unfold ETyping.declared_constant in *.
       rewrite isdecl0 in isdecl.
       noconf isdecl.
-      rewrite H0 in H.
-      noconf H.
+      rewrite e0 in e.
+      noconf e.
       now apply IHev in ev'.
     + easy.
   - depelim ev'.
@@ -530,9 +539,9 @@ Proof.
     + apply IHev1 in ev'1.
       apply IHev2 in ev'2.
       subst.
-      rewrite isFixApp_mkApps in H by easy.
-      cbn in H.
-      now rewrite orb_true_r in H.
+      rewrite isFixApp_mkApps in i by easy.
+      cbn in *.
+      now rewrite orb_true_r in i.
     + apply IHev1 in ev'1.
       apply IHev2 in ev'2.
       now subst.
